### Finding the Slope

Let's say we have a problem with two points:
$$
(1,0)(0,-1) \label{FindSlope1}
$$
And it states to find the slope given these two points. To do this, remember the Slope Formula for a line:
$$
m = \frac{\text{rise}}{\text{run}} = \frac{y_{2} - y_{1}}{x_{2} - x_{1}} \label{SlopeFormula}
$$
Also remember a point has an $xy$-pair such as ($x,y$). Let's label ($\ref{FindSlope1}$) with the first point having an $xy$-pair of ($x_{1},y_{1}$) while the second point has ($x_{2},y_{2}$):
$$
\begin{equation}
(\underbrace{1}_\text{x_1} ,\underbrace{0}_\text{y1} )(\underbrace{0}_\text{x2} ,\underbrace{-1}_\text{y2} ) \label{FindSlope2}
\end{equation}
$$
Notice how the labels $x_{1}$, $y_{1}$, $x_{2}$, $y_{2}$ are underneath the numbers? It is recommended to do this so you could keep track and make less mistakes. With the labeling now complete, use the Slope Formula from ($\ref{SlopeFormula}$) to plug in the numbers from ($\ref{FindSlope2}$) into the correct labels:
$$
\begin{align}
m = \frac{y_{2} - y_{1}}{x_{2} - x_{1}} = \frac{-1 - 0}{0 - 1} \\
= \frac{-1}{-1} \xrightarrow{\text{becomes positive}} \frac{1}{1} \label{FindSlope3} \\
\boxed{m = 1}
\end{align}
$$
Notice how on ($\ref{FindSlope3}$) the two negatives on top and bottom give you a positive since dividing two negatives gives you a positive.

And that is how you Find the Slope of a Line!

### Substitution Method

For the Substitution Method, there needs to be at least 2 equations, and they could have have two variables such as $x$ and $y$. NOTE: The variables does not need to be in $x$ or $y$, but they could be any type of letter!

Either of the 2 equations could be in a form where both variables are by each other: $x + y = 10$, $y - x = -1$, and so on. The variables could be opposite of each other where one is on the left side of the equal sign while the other is on the right side: $x = y$, $y - 5 = x$, $x + 1 = 2 + y$, and so on.

Lastly, the equations might only have one variable equal to a number: $x = 1$, $y = 0$, and so on.

Let's say we have a problem like so:
$$
\begin{alignat}{2}
x + y = 2 \label{Sub1} \xrightarrow{\text{This is (7)}} \\
4x - y = 8 \label{Sub2} \xrightarrow[\text{This is (8)}]{}
\end{alignat}
$$
To solve this Systems of Equations by using the Substitution Method, you have to isolate one of the variables from either ($\ref{Sub1}$) or ($\ref{Sub2}$). Let's pick ($\ref{Sub1}$) since that looks the easiest, and let's start isolating the variable $y$ by subtracting $x$ from both sides:
$$
\begin{align}
x - x + y = 2 - x \\
y = 2 - x \label{Sub4}
\end{align}
$$
The variable $y$ is now isolated, and now let's plug ($\ref{Sub4}$) into ($\ref{Sub2}$) in order to solve for $x$:
$$
4x - (2 - x) = 8 \label{Sub5}
$$
Notice how on ($\ref{Sub5}$) the $y$ gets replaced with ($\ref{Sub4}$) since that is what $y$ equals to, and also noticed how on ($\ref{Sub5}$) the parenthesis $()$ is surrounding $2 - x$? Whenever you replace a variable with an equation, you always put that equation in parenthesis in order to avoid getting the wrong answer! IMPORTANT: Always put parenthesis no what it is such as $2 - x$, or a single variable like $x$, or a number with no variable like $2$, or a single variable that is negative like $-x$, and so on.

Let's continue by distributing the minus sign in front of the left parenthesis onto $2$ and $-x$:
$$
4x - 2 - - x = 8 \\
4x - 2 + x = 8 \label{Sub6}
$$
Notice how on ($\ref{Sub6}$) the $x$ becomes a **_positive_** since the two negatives give you a minus sign. Let's continue where on the left side of the equal sign we have *like terms* of $4x$ and $x$, and combining them gives you $4x + x = 5x$. This gives you $5x - 2 = 8$. Now, you need $x$ to be by itself and to do that is by first adding $2$ to both sides of the equal sign, and we *add* since to get rid of $-2$ is by taking its *opposite* which is $+2$:
$$
5x - 2 + 2 = 8 + 2 \\
5x = 10
$$
Now, you have $x$ being multiplied by $5$. To get rid of $5$,  take the *reciprocal* of $5$ on both sides of the equation. Another way to think about this is since $x$ is being *multiplied* by $5$, take the opposite of *multiplication* which is *division*:
$$
\begin{align}
\frac{5x}{5} = \frac{10}{5} \\
x = \frac{10}{5} \\
x = 2 \label{Sub10}
\end{align}
$$
Almost done! With ($\ref{Sub10}$), we could plug this into either ($\ref{Sub1}$) or ($\ref{Sub2}$) to solve for $y$. Let's pick ($\ref{Sub1}$) since that looks pretty easy, and remember to put it into parenthesis:
$$
\begin{align}
x + y = 2 \xrightarrow{\text{becomes}} (2) + y = 2 \\
2 + y = 2 \xrightarrow{\text{subtract 2 to both sides}} 2 - 2 + y = 2 - 2 \\
y = 2 - 2 \\
y = 0
\end{align}
$$
THIS IS NOT THE FINAL ANSWER! Your teacher is going to want to have in *point form* such as $(x,y)$. With $x = 2$ and $y = 0$, the final answer is:
$$
(x,y) = \boxed{(2,0)}
$$
That is how you do the Substitution Method!

### Graphing Systems of Equations

To graph Systems of Equations, lets use the equations ($\ref{Sub1}$) and ($\ref{Sub2}$) from the Substitution Method section. Now, to graph these two equations, one of the methods to use is finding the x and y intercepts. Once you find the x and y intercepts for one line, you can plot them and draw a line through those two points. After that, do the same procedure for the second line.

For our first line, we'll start with equation ($\ref{Sub1}$). The first step is to set either $x$ or $y$ equal to $0$, and then solve for the either variable. In this case, let's set $x$ equal to $0$:
$$
x + y = 2 \xrightarrow{\text{x becomes 0}} 0 + y = 2 \xrightarrow{\text{0 + y = y}} y = 2 \label{YInt1}
$$
From ($\ref{YInt1}$), we have $y = 2$ with $x = 0$, and thus our y-intercept in point form is ($x,y$) $=$ ($0,2$). This is for equation ($\ref{Sub1}$), and also remember that you need to have it in point form or your teacher is going to dock some points. Now, lets find the x-intercept on ($\ref{Sub1}$) by using a similar procedure, but this time setting $y = 0$:
$$
x + y = 2 \xrightarrow{\text{y becomes 0}} x + 0 = 2 \xrightarrow{\text{x + 0 = x}} x = 2 \label{XInt1}
$$
From ($\ref{XInt1}$), we have an x-intercept of ($x,y$) $=$ ($2, 0$) in point form where $x = 2$ and $y = 0$. With this, we could now plot these points on a graph for equation ($\ref{Sub1}$), and we'll do it step-by-step on plotting them. Lastly, here are x-intercept, y-intercept, and equation ($\ref{Sub1}$) as reference:
$$
\begin{align*}
x + y = 2, \quad \text{x-int: } (2, 0), \quad \text{y-int: } (0, 2)
\end{align*}
$$
First, start from the center $0$ and plot the x-intercept by moving $2$ to the right for $x$, and since $y$ is $0$ then it stays put without going up or down:

![x-intercept for (7)](C:\Users\mrdrp\Documents\Sanger-High-School\img\integrated-math-1\weeks5-6_2020-05-22\x1-intercept.png)

Now, plot the y-intercept by starting at the center $0$ and do not move left or right since $x = 0$, but move up to the number $2$ since $y = 2$:

![y-intercept for (7)](C:\Users\mrdrp\Documents\Sanger-High-School\img\integrated-math-1\weeks5-6_2020-05-22\y1-intercept.png)

With a straight edge like a ruler or an ID card, draw a line through these two points:

![A line through the x-intercept and y-intercept for (7)](C:\Users\mrdrp\Documents\Sanger-High-School\img\integrated-math-1\weeks5-6_2020-05-22\line-1.png)

Next, use equation ($\ref{Sub1}$) to label the line you just drew. NOTE: Do not label how it is going to be shown, but label the equation next to the line:

![Equation (7) line with labeling](C:\Users\mrdrp\Documents\Sanger-High-School\img\integrated-math-1\weeks5-6_2020-05-22\line-1-label.png)